add Stack.args and Stack.tail_region, refactor distance

StackLean/Definitions.lean
@@ -1,3 +1,9 @@
+import Init.Data.List.Lemmas
+import Init.Data.List.Nat.Sublist
+import Init.Data.List.Nat.TakeDrop
+import Mathlib.Data.List.TakeDrop
+import Mathlib.Data.List.Lemmas
+import Mathlib.Data.List.Lemmas
 import Mathlib.Data.Nat.Basic
 import Aesop
 
@@ -45,6 +51,144 @@ structure Target where
   size : { n : ℕ // n ≥ args.length + liveOut.count }
 
 def Target.vars (target : Target) : LSet Var := target.args.vars ∪ target.liveOut
+
+@[simp]
+abbrev Target.tail_length (target : Target) := target.size - target.args.length
+
+--- Stack Args ---
+
+@[simp, reducible]
+def Stack.args (stack : Stack) (target : Target) : Stack :=
+  if stack.length > target.size
+  then
+    stack
+      -- drop the excess
+      |> List.drop (stack.length - target.size)
+      -- take the args
+      |> List.take target.args.length
+  else
+    -- take whatever stack region we have above the tail
+    stack.take (stack.length - target.tail_length)
+
+@[simp]
+abbrev example_target (args_sz : ℕ) (total_sz : ℕ) (hsz : total_sz ≥ args_sz := by omega) : Target
+  := ⟨List.replicate args_sz (.Lit 1), LSet.ofList [], ⟨total_sz, by simp [LSet.ofList]; grind⟩⟩
+
+example : Stack.args [.Lit 3, .Lit 4, .Lit 5] (example_target 2 4) = [.Lit 3]
+  := by simp_all [Stack.args]
+
+example : Stack.args [.Lit 1, .Lit 2, .Lit 3, .Lit 4, .Lit 5] (example_target 2 3) = [.Lit 3, .Lit 4]
+  := by simp_all [Stack.args]
+
+example : Stack.args [.Lit 1, .Lit 2, .Lit 3, .Lit 4, .Lit 5] (example_target 1 4) = [.Lit 2]
+  := by simp_all [Stack.args]
+
+example : Stack.args [.Lit 1, .Lit 2, .Lit 3, .Lit 4, .Lit 5] (example_target 2 2) = [.Lit 4, .Lit 5]
+  := by simp_all [Stack.args]
+
+example : Stack.args [.Lit 1, .Lit 2, .Lit 3, .Lit 4, .Lit 5] (example_target 2 5) = [.Lit 1, .Lit 2]
+  := by simp_all [Stack.args]
+
+example : Stack.args [.Lit 1, .Lit 2, .Lit 3, .Lit 4, .Lit 5] (example_target 2 6) = [.Lit 1]
+  := by simp_all [Stack.args]
+
+example : Stack.args [.Lit 1, .Lit 2, .Lit 3, .Lit 4, .Lit 5] (example_target 7 10) = [.Lit 1, .Lit 2]
+  := by simp_all [Stack.args]
+
+example : Stack.args [.Lit 1, .Lit 2, .Lit 3, .Lit 4, .Lit 5] (example_target 1 10) = []
+  := by simp_all [Stack.args]
+
+@[simp]
+theorem args_le_target_args (stack : Stack) (target : Target)
+  : (stack.args target).length ≤ target.args.length := by
+    simp_all [Stack.args]
+    grind only [= List.length_drop, = List.length_take, = Nat.min_def, cases Or]
+
+-- if we prepend the target args any base with length ≤ the tail length, and
+-- then take the args of that stack relative to the target, the result is the target.args
+theorem args_concat_base_leq
+  (base : Stack) (target : Target) (hsz : base.length ≤ target.tail_length)
+    : let input := target.args ++ base
+      input.args target = target.args.take (input.length - target.tail_length)
+  := by
+    simp_all [Stack.args]
+    split_ifs
+    · grind
+    · simp_all
+
+-- if we prepend the target args any base with length = the tail length, and
+-- then prepend any stack to that, the args of the result relative to the target is the target.args
+theorem args_concat_top_base_eq
+  (top : Stack) (base : Stack) (target : Target) (hsz : base.length = target.tail_length)
+    : let input := top ++ target.args ++ base
+      input.args target = target.args
+  := by
+    simp_all [Stack.args]
+    split_ifs
+    · have :
+        (top.length +
+          (target.args.length + (↑target.size - target.args.length))
+        - ↑target.size) = top.length := by grind
+      simp_all
+    · have : top.length = 0 := by omega
+      simp_all
+
+--- Stack Tail ---
+
+@[simp, reducible]
+def Stack.tail_region (stack : Stack) (target : Target) : Stack :=
+    if stack.length > target.size
+    then
+      -- drop the excess and the args
+      stack.drop ((stack.length - target.size) + target.args.length)
+    else
+      -- drop whatever stack region we have above the tail
+      let tail_length := target.size - target.args.length
+      stack.drop (stack.length - tail_length)
+
+example : Stack.tail_region [.Lit 3, .Lit 4, .Lit 5] (example_target 2 4) = [.Lit 4, .Lit 5]
+  := by simp_all [Stack.tail_region]
+
+example : Stack.tail_region [.Lit 1, .Lit 2, .Lit 3, .Lit 4, .Lit 5] (example_target 2 3) = [.Lit 5]
+  := by simp_all [Stack.tail_region]
+
+example : Stack.tail_region [.Lit 1, .Lit 2, .Lit 3, .Lit 4, .Lit 5] (example_target 1 4) = [.Lit 3, .Lit 4, .Lit 5]
+  := by simp_all [Stack.tail_region]
+
+example : Stack.tail_region [.Lit 1, .Lit 2, .Lit 3, .Lit 4, .Lit 5] (example_target 2 2) = []
+  := by simp_all [Stack.tail_region]
+
+example : Stack.tail_region [.Lit 1, .Lit 2, .Lit 3, .Lit 4, .Lit 5] (example_target 2 5) = [.Lit 3, .Lit 4, .Lit 5]
+  := by simp_all [Stack.tail_region]
+
+example : Stack.tail_region [.Lit 1, .Lit 2, .Lit 3, .Lit 4, .Lit 5] (example_target 2 6) = [.Lit 2, .Lit 3, .Lit 4, .Lit 5]
+  := by simp_all [Stack.tail_region]
+
+example : Stack.tail_region [.Lit 1, .Lit 2, .Lit 3, .Lit 4, .Lit 5] (example_target 7 10) = [.Lit 3, .Lit 4, .Lit 5]
+  := by simp_all [Stack.tail_region]
+
+example : Stack.tail_region [.Lit 1, .Lit 2, .Lit 3, .Lit 4, .Lit 5] (example_target 1 10) = [.Lit 1, .Lit 2, .Lit 3, .Lit 4, .Lit 5]
+  := by simp_all [Stack.tail_region]
+
+theorem stack_tail_le_target_tail_length (stack : Stack) (target : Target) : (stack.tail_region target).length ≤ target.tail_length := by
+  simp_all [Stack.tail_region]
+  split_ifs <;> grind only [= List.length_drop, cases Or]
+
+theorem stack_tail_eq_stack_length_leq_tail_length
+  (stack : Stack) (target : Target)
+  (hlen : stack.length ≤ target.tail_length)
+    : stack.tail_region target = stack := by
+  simp_all [Stack.tail_region]
+  intro hsz
+  grind
+
+theorem stack_tail_eq_stack_length_gt_tail_length
+  (stack : Stack) (target : Target)
+  (hlen : stack.length > target.tail_length)
+    : stack.tail_region target = stack.drop (stack.length - target.tail_length) := by
+  simp_all [Stack.tail_region]
+  intro hsz
+  grind
 
 --- Traces ---
 
